src/Core_Erlang_Weak_Equivalence.v
@@ -580,7 +580,7 @@ End helpers.
 
 Section equivalence_relation.
 
-Theorem weak_refl e :
+Theorem weak_refl {e} :
   weakly_equivalent e e.
 Proof.
   unfold weakly_equivalent. split; intros.
@@ -588,7 +588,7 @@ Proof.
   eexists. split. apply H. apply Permutation_refl.
 Qed.
 
-Theorem weak_sym e1 e2 :
+Theorem weak_sym {e1 e2} :
   weakly_equivalent e1 e2
 ->
   weakly_equivalent e2 e1.
@@ -598,7 +598,7 @@ Proof.
   destruct H. apply H in H0. exact H0.
 Qed.
 
-Theorem weak_trans e1 e2 e3 :
+Theorem weak_trans {e1 e2 e3} :
   weakly_equivalent e1 e2 -> weakly_equivalent e2 e3
 ->
   weakly_equivalent e1 e3.
@@ -611,7 +611,7 @@ Proof.
     split. exact H1. eapply Permutation_trans. exact H4. exact H5.
 Qed.
 
-Theorem weak_single_refl e :
+Theorem weak_single_refl {e} :
   weakly_equivalent_single e e.
 Proof.
   unfold weakly_equivalent_single. split; intros.
@@ -619,7 +619,7 @@ Proof.
   eexists. split. apply H. apply Permutation_refl.
 Qed.
 
-Theorem weak_single_sym e1 e2 :
+Theorem weak_single_sym {e1 e2} :
   weakly_equivalent_single e1 e2
 ->
   weakly_equivalent_single e2 e1.
@@ -629,7 +629,7 @@ Proof.
   destruct H. apply H in H0. exact H0.
 Qed.
 
-Theorem weak_single_trans e1 e2 e3 :
+Theorem weak_single_trans {e1 e2 e3} :
   weakly_equivalent_single e1 e2 -> weakly_equivalent_single e2 e3
 ->
   weakly_equivalent_single e1 e3.
@@ -646,7 +646,381 @@ End equivalence_relation.
 
 Section congruence.
 
-Theorem ESeq_congr_weak e1 e2 e1' e2' :
+Theorem ECons_weak_congr hd tl : forall hd' tl',
+  weakly_equivalent hd hd' -> weakly_equivalent tl tl'
+->
+  weakly_equivalent_single (ECons hd tl) (ECons hd' tl').
+Proof.
+  assert (A : forall hd hd' tl tl' env id eff id' res eff',
+    weakly_equivalent hd hd' -> weakly_equivalent tl tl' ->
+    | env, id, ECons hd tl, eff | -s> |id', res, eff'|
+  ->
+    (exists eff'', | env, id, ECons hd' tl', eff | -s> |id', res, eff''| /\ Permutation eff' eff'')
+  ). {
+    intros. unfold weakly_equivalent in H, H0. destruct H, H0. inversion H1; subst.
+    * apply effect_extension_expr in H8 as H8'. destruct H8'. subst.
+      apply effect_extension_expr in H13 as H13'. destruct H13'. subst.
+      pose (P := H0 _ _ _ _ _ _ H8). destruct P, H4.
+      apply effect_extension_expr in H4 as H4'. destruct H4'. subst.
+      apply effectlist_irrelevant_expr with (eff0 := eff ++ x2) in H13.
+      pose (P := H _ _ _ _ _ _ H13). destruct P, H6.
+      apply effect_extension_expr in H6 as H6'. destruct H6'. subst.
+      exists ((eff ++ x2) ++ x3). split. eapply eval_cons.
+      - exact H4.
+      - exact H6.
+      - rewrite <- app_assoc, <- app_assoc.
+        apply Permutation_app_head. apply Permutation_app_inv_l in H5.
+        apply Permutation_app. exact H5.
+        apply Permutation_app_inv_l in H7. exact H7.
+    * apply effect_extension_expr in H12 as H12'. destruct H12'. subst.
+      pose (P := H0 _ _ _ _ _ _ H12). destruct P, H4.
+      apply effect_extension_expr in H4 as H4'. destruct H4'. subst.
+      exists (eff ++ x1). split.
+      - eapply eval_cons_tl_ex. exact H4.
+      - apply Permutation_app_head. apply Permutation_app_inv_l in H5. exact H5.
+    * apply effect_extension_expr in H8 as H8'. destruct H8'. subst.
+      apply effect_extension_expr in H13 as H13'. destruct H13'. subst.
+      pose (P := H0 _ _ _ _ _ _ H8). destruct P, H4.
+      apply effect_extension_expr in H4 as H4'. destruct H4'. subst.
+      apply effectlist_irrelevant_expr with (eff0 := eff ++ x2) in H13.
+      pose (P := H _ _ _ _ _ _ H13). destruct P, H6.
+      apply effect_extension_expr in H6 as H6'. destruct H6'. subst.
+      exists ((eff ++ x2) ++ x3). split. eapply eval_cons_hd_ex.
+      - exact H4.
+      - exact H6.
+      - rewrite <- app_assoc, <- app_assoc.
+        apply Permutation_app_head. apply Permutation_app_inv_l in H5.
+        apply Permutation_app. exact H5.
+        apply Permutation_app_inv_l in H7. exact H7.
+  }
+  split; intros.
+  * eapply A. exact H. exact H0. exact H1.
+  * eapply A. exact (weak_sym H). exact (weak_sym H0). exact H1.
+Qed.
+
+Theorem ETuple_weak_congr (l : list Expression) : forall (l' : list Expression),
+  length l = length l' ->
+  (forall i, i < length l -> weakly_equivalent (nth i l ErrorExp) (nth i l' ErrorExp))
+->
+  weakly_equivalent_single (ETuple l) (ETuple l').
+Proof.
+  assert (A : forall (l l' : list Expression) env id eff id' res eff',
+    length l = length l' ->
+    (forall i, i < length l -> weakly_equivalent (nth i l ErrorExp) (nth i l' ErrorExp))
+    ->
+    |env, id, ETuple l, eff| -s> |id', res, eff'|
+    ->
+    |env, id, ETuple l', eff| -s> |id', res, eff'|). {
+  intros. unfold weakly_equivalent, weakly_equivalent_single in *.
+  * inversion H1; subst; rewrite H in *.
+    - eapply eval_tuple.
+      + exact H3.
+      + exact H4.
+      + exact H5.
+      + intros. pose (H6 i H2). apply H0 in e. 2: auto. auto.
+      + auto.
+      + auto.
+    - eapply eval_tuple_ex.
+      + exact H3.
+      + reflexivity.
+      + exact H5.
+      + exact H6.
+      + intros. pose (H7 j H2). apply H0 in e. 2: lia. auto.
+      + apply H0 in H10. auto. lia.
+  }
+  split; intros.
+  * eapply A. exact H. auto. auto.
+  * eapply A. symmetry. exact H. intros. rewrite <- H in *.
+    apply weak_sym. auto. auto.
+Qed.
+
+Theorem ECall_weak_congr (f : string) (l : list Expression) : forall (l' : list Expression),
+  length l = length l' ->
+  (forall i, i < length l -> weakly_equivalent (nth i l ErrorExp) (nth i l' ErrorExp))
+->
+  weakly_equivalent_single (ECall f l) (ECall f l').
+Proof.
+  assert (A : forall f (l l' : list Expression) env id eff id' res eff',
+  length l = length l' ->
+  (forall i, i < length l -> weakly_equivalent (nth i l ErrorExp) (nth i l' ErrorExp))
+  ->
+  |env, id, ECall f l, eff| -s> |id', res, eff'|
+  ->
+  |env, id, ECall f l', eff| -s> |id', res, eff'|). {
+  intros. unfold weakly_equivalent, weakly_equivalent_single in *.
+  * inversion H1; subst; rewrite H in *.
+    - eapply eval_call.
+      + exact H4.
+      + exact H5.
+      + exact H6.
+      + intros. pose (H7 i H2). apply H0 in e. 2: auto. auto.
+      + auto.
+      + auto.
+    - eapply eval_call_ex.
+      + exact H4.
+      + reflexivity.
+      + exact H6.
+      + exact H7.
+      + intros. pose (H10 j H2). apply H0 in e. 2: lia. auto.
+      + apply H0 in H15. auto. lia.
+  }
+  split; intros.
+  * eapply A. exact H. auto. auto.
+  * eapply A. symmetry. exact H. intros. rewrite <- H in *.
+    apply weak_sym. auto. auto.
+Qed.
+
+Theorem EPrimOp_weak_congr (f : string) (l : list Expression) : forall (l' : list Expression),
+  length l = length l' ->
+  (forall i, i < length l -> weakly_equivalent (nth i l ErrorExp) (nth i l' ErrorExp))
+->
+  weakly_equivalent_single (EPrimOp f l) (EPrimOp f l').
+Proof.
+  assert (A : forall f (l l' : list Expression) env id eff id' res eff',
+  length l = length l' ->
+  (forall i, i < length l -> weakly_equivalent (nth i l ErrorExp) (nth i l' ErrorExp))
+  ->
+  |env, id, EPrimOp f l, eff| -s> |id', res, eff'|
+  ->
+  |env, id, EPrimOp f l', eff| -s> |id', res, eff'|). {
+  intros. unfold weakly_equivalent, weakly_equivalent_single in *.
+  * inversion H1; subst; rewrite H in *.
+    - eapply eval_primop.
+      + exact H4.
+      + exact H5.
+      + exact H6.
+      + intros. pose (H7 i H2). apply H0 in e. 2: auto. auto.
+      + auto.
+      + auto.
+    - eapply eval_primop_ex.
+      + exact H4.
+      + reflexivity.
+      + exact H6.
+      + exact H7.
+      + intros. pose (H10 j H2). apply H0 in e. 2: lia. auto.
+      + apply H0 in H15. auto. lia.
+  }
+  split; intros.
+  * eapply A. exact H. auto. auto.
+  * eapply A. symmetry. exact H. intros. rewrite <- H in *.
+    apply weak_sym. auto. auto.
+Qed.
+
+Theorem EApp_weak_congr (exp : Expression) (l : list Expression) : forall (exp' : Expression) (l' : list Expression),
+  length l = length l' ->
+  weakly_equivalent exp exp' ->
+  (forall i, i < length l -> weakly_equivalent (nth i l ErrorExp) (nth i l' ErrorExp))
+->
+  weakly_equivalent_single (EApp exp l) (EApp exp' l').
+Proof.
+  assert (A : forall exp exp' (l l' : list Expression) env id eff id' res eff',
+    length l = length l' ->
+    weakly_equivalent exp exp' ->
+    (forall i, i < length l -> weakly_equivalent (nth i l ErrorExp) (nth i l' ErrorExp))
+    ->
+    |env, id, EApp exp l, eff| -s> |id', res, eff'|
+    ->
+    |env, id, EApp exp' l', eff| -s> |id', res, eff'|).
+  {
+    unfold weakly_equivalent.
+    intros. remember (EApp exp0 l0) as appl.
+    induction H2; inversion Heqappl; subst.
+    * eapply eval_app; rewrite H in *.
+      - exact H2.
+      - apply H0. exact H3.
+      - auto.
+      - exact H5.
+      - exact H6.
+      - intros. pose (H7 i H9). apply H1. auto. auto.
+      - auto.
+    * eapply eval_app_closure_ex. apply H0. exact H2.
+    * eapply eval_app_param_ex; rewrite H in *.
+      - exact H2.
+      - reflexivity.
+      - exact H4.
+      - exact H5.
+      - apply H0. auto. exact H6.
+      - intros. pose (H7 j H3). apply H1. lia. auto.
+      - apply H1. lia. auto.
+    * eapply eval_app_badfun_ex; rewrite H in *.
+      - exact H2.
+      - exact H3.
+      - exact H4.
+      - apply H0. auto. exact H5.
+      - intros. pose (H6 j H8). apply H1. lia. auto.
+      - congruence.
+      - auto.
+      - auto.
+    * eapply eval_app_badarity_ex; rewrite H in *.
+      - exact H2.
+      - exact H3.
+      - exact H4.
+      - apply H0. auto. exact H5.
+      - intros. pose (H6 j H8). apply H1. lia. auto.
+      - congruence.
+      - auto.
+      - auto.
+  }
+  intros. split.
+  * apply A; auto.
+  * apply A; try lia.
+    apply weak_sym. auto.
+    intros. apply weak_sym. apply H1. lia.
+Qed.
+
+Theorem case_weak_congr_helper (l l' : list (list Pattern * Expression * Expression)) vals j gg ee bb:
+length l = length l' ->
+((forall i, i < length l -> weakly_equivalent (nth i (map snd l) ErrorExp)
+                                                   (nth i (map snd l') ErrorExp) /\
+                             weakly_equivalent (nth i (map snd (map fst l)) ErrorExp)
+                                                   (nth i (map snd (map fst l')) ErrorExp)
+                   /\ nth i (map fst (map fst l)) [] = nth i (map fst (map fst l')) [])) ->
+ match_clause vals l j = Some (gg, ee, bb)
+->
+ match_clause vals l' j = Some (nth j (map snd (map fst l')) ErrorExp, nth j (map snd l') ErrorExp, bb).
+Proof.
+  generalize dependent l'. generalize dependent j.
+  induction l; intros.
+  * inversion H1.
+  * pose (element_exist _ _ H). destruct e. destruct H2. subst.
+    inversion H.
+    destruct j.
+    - simpl. simpl in H1. destruct a, p, x, p.
+      pose (H0 0 (Nat.lt_0_succ _)). destruct a. destruct H4.
+      simpl in H2, H4, H5. subst.
+      destruct (match_valuelist_to_patternlist vals l1).
+      + simpl. inversion H1. auto.
+      + congruence.
+    - simpl. simpl in H1. destruct a, p, x, p.
+      apply IHl. auto.
+      intros. epose (H0 (S i) _). simpl in a. exact a. Unshelve. 2: simpl; lia.
+      auto.
+Qed.
+
+Theorem ECase_weak_congr (exp : Expression) (l : list (list Pattern * Expression * Expression)) : forall (exp' : Expression) (l' : list (list Pattern * Expression * Expression)),
+  length l = length l' ->
+  weakly_equivalent exp exp' ->
+  (forall i, i < length l -> weakly_equivalent (nth i (map snd l) ErrorExp)
+                                                   (nth i (map snd l') ErrorExp) /\
+                             weakly_equivalent (nth i (map snd (map fst l)) ErrorExp)
+                                                   (nth i (map snd (map fst l')) ErrorExp)
+                   /\ nth i (map fst (map fst l)) [] = nth i (map fst (map fst l')) [])
+->
+  weakly_equivalent_single (ECase exp l) (ECase exp' l').
+Proof.
+  intros. unfold weakly_equivalent, weakly_equivalent_single in *.
+  split; intros; inversion H2; subst.
+  * eapply eval_case; rewrite H in *.
+    - apply H0. exact H5.
+    - exact H6.
+    - apply case_congr_helper with (l' := l') in H7.
+      3: unfold weakly_equivalent; rewrite H; exact H1.
+      exact H7.
+      auto.
+    - intros. assert (match_clause vals l' j = Some (gg, ee, bb)). { auto. }
+      apply match_clause_ith in H9. destruct H9. destruct H10. subst.
+      apply case_congr_helper with (l' := l) in H4. 2: auto.
+      pose (H8 j H3 _ _ _ H4). epose (H1 j _). Unshelve. 3: lia. destruct a.
+      apply H10. exact e.
+      intros. split. 2: split.
+      + apply weak_sym. epose (H1 i0 _). Unshelve. 2: lia. destruct a.
+        unfold weakly_equivalent.
+        intros. apply H10.
+      + apply weak_sym. epose (H1 i0 _). Unshelve. 2: lia. destruct a.
+        unfold weakly_equivalent.
+        intros. apply H12.
+      + epose (H1 i0 _). Unshelve. 2: lia. destruct a.
+        destruct H12. auto.
+    - apply match_clause_ith in H7. destruct H7, H4. subst.
+      apply H1. auto. auto.
+    - apply match_clause_ith in H7. destruct H7, H4. subst.
+      apply H1. auto. auto.
+  * eapply eval_case_pat_ex. apply H0. auto.
+  * eapply eval_case_clause_ex.
+    - apply H0. exact H7.
+    - intros. assert (match_clause vals l' j = Some (gg, ee, bb)). { auto. }
+      apply match_clause_ith in H5. destruct H5. destruct H6. subst.
+      apply case_congr_helper with (l' := l) in H4.
+      rewrite H in *. 2: auto.
+      pose (H12 j H3 _ _ _ H4). epose (H1 j _). Unshelve. 3: lia. destruct a.
+      apply H6. exact e.
+      intros. split. 2: split.
+      + apply weak_sym. epose (H1 i _). Unshelve. 2: lia. destruct a.
+        unfold weakly_equivalent.
+        intros. apply H6.
+      + apply weak_sym. epose (H1 i _). Unshelve. 2: lia. destruct a.
+        unfold weakly_equivalent.
+        intros. apply H8.
+      + epose (H1 i _). Unshelve. 2: lia. destruct a.
+        destruct H8. auto.
+  * eapply eval_case; rewrite <- H in *.
+    - apply H0. exact H5.
+    - exact H6.
+    - apply case_congr_helper with (l' := l) in H7. 2: lia.
+      exact H7.
+      rewrite <- H. intros.
+      split. 2: split.
+      + apply weak_sym. pose (H1 i0 H3). unfold weakly_equivalent.
+        apply a.
+      + apply weak_sym. pose (H1 i0 H3). unfold weakly_equivalent.
+        apply a.
+      + pose (H1 i0 H3). unfold weakly_equivalent. destruct a. destruct H9.
+        symmetry. apply H10.
+    - intros. assert (match_clause vals l j = Some (gg, ee, bb)). { auto. }
+      apply match_clause_ith in H9. destruct H9. destruct H10. subst.
+      apply case_congr_helper with (l' := l') in H4. 2: auto.
+      pose (H8 j H3 _ _ _ H4). epose (H1 j _). Unshelve. 3: lia. destruct a.
+      apply H10. exact e.
+      intros. split. 2: split.
+      + apply weak_sym. epose (H1 i0 _). Unshelve. 2: lia. destruct a.
+        unfold weakly_equivalent. symmetry.
+        intros. apply H10.
+      + apply weak_sym. epose (H1 i0 _). Unshelve. 2: lia. destruct a.
+        unfold weakly_equivalent.
+        intros. symmetry. apply H12.
+      + epose (H1 i0 _). Unshelve. 2: lia. destruct a.
+        destruct H12. auto.
+    - apply match_clause_ith in H7. destruct H7, H4. subst.
+      apply H1. auto. auto.
+    - apply match_clause_ith in H7. destruct H7, H4. subst.
+      apply H1. auto. auto.
+  * eapply eval_case_pat_ex. apply H0. auto.
+  * eapply eval_case_clause_ex.
+    - apply H0. exact H7.
+    - intros. assert (match_clause vals l j = Some (gg, ee, bb)). { auto. }
+      apply match_clause_ith in H5. destruct H5. destruct H6. subst.
+      apply case_congr_helper with (l' := l') in H4. 2: auto.
+      rewrite H in *.
+      pose (H12 j H3 _ _ _ H4). epose (H1 j _). Unshelve. 3: lia. destruct a.
+      apply H6. exact e.
+      intros. split. 2: split.
+      + apply weak_sym. epose (H1 i _). Unshelve. 2: lia. destruct a.
+        unfold weakly_equivalent.
+        intros. symmetry. apply H6.
+      + apply weak_sym. epose (H1 i _). Unshelve. 2: lia. destruct a.
+        unfold weakly_equivalent.
+        intros. symmetry. apply H8.
+      + epose (H1 i _). Unshelve. 2: lia. destruct a.
+        destruct H8. auto.
+Qed.
+
+Theorem ELet_weak_congr (e1 e2 : Expression) vl : forall (e1' e2' : Expression),
+  weakly_equivalent e1 e1' ->
+  weakly_equivalent e2 e2'
+->
+  weakly_equivalent_single (ELet vl e1 e2) (ELet vl e1' e2').
+Proof.
+  intros. unfold weakly_equivalent, weakly_equivalent_single in *.
+  split; intros.
+  * inversion H1; subst.
+    - eapply eval_let. apply H. exact H7. auto. apply H0. exact H13.
+    - eapply eval_let_ex. apply H. auto.
+  * inversion H1; subst.
+    - eapply eval_let. apply H. exact H7. auto. apply H0. exact H13.
+    - eapply eval_let_ex. apply H. auto.
+Qed.
+
+Theorem ESeq_weak_congr e1 e2 e1' e2' :
   weakly_equivalent e1 e1' -> weakly_equivalent e2 e2'
 ->
   weakly_equivalent_single (ESeq e1 e2) (ESeq e1' e2').
@@ -677,6 +1051,146 @@ Proof.
         ** apply Permutation_app_tail. auto.
     - subst. apply H in H10. destruct H10.
       eexists. split. eapply eval_seq_ex. apply H2. apply H2.
+Qed.
+
+Theorem ELetRec_weak_congr (exp : Expression) l : forall (exp' : Expression),
+  weakly_equivalent exp exp'
+->
+  weakly_equivalent_single (ELetRec l exp) (ELetRec l exp').
+Proof.
+  intros. unfold weakly_equivalent, weakly_equivalent_single in *.
+  split; intros.
+  * inversion H0. subst. eapply eval_letrec. apply H. exact H9.
+  * inversion H0. subst. eapply eval_letrec. apply H. exact H9.
+Qed.
+
+Theorem EMap_weak_congr (l : list (Expression * Expression)) : 
+  forall (l' : list (Expression * Expression)),
+  length l = length l' ->
+  (let exps := make_map_exps l in
+   let exps' := make_map_exps l' in
+  forall i, i < length exps -> weakly_equivalent (nth i exps ErrorExp) (nth i exps' ErrorExp))
+->
+  weakly_equivalent_single (EMap l) (EMap l').
+Proof.
+  assert (A :
+    forall (l l' : list (Expression * Expression)) env id eff eff' id' res,
+    length l = length l' ->
+    (let exps := make_map_exps l in
+      let exps' := make_map_exps l' in
+       forall i, i < length exps -> weakly_equivalent (nth i exps ErrorExp) (nth i exps' ErrorExp)) ->
+    |env, id, EMap l, eff | -s> |id', res, eff'|
+    ->
+    |env, id, EMap l', eff | -s> |id', res, eff' |
+  ). {
+  intros. unfold weakly_equivalent, weakly_equivalent_single in *.
+  * inversion H1; subst; rewrite H in *.
+    - unfold exps, vals in *.
+      eapply eval_map.
+      + exact H3.
+      + exact H4.
+      + exact H5.
+      + exact H6.
+      + intros. rewrite length_make_map_exps in H2, H7. rewrite H in H7.
+        pose (H7 i H2). apply H0 in e. exact e.
+        rewrite length_make_map_exps. lia.
+      + exact H8.
+      + auto.
+      + auto.
+      + auto.
+    - unfold exps, vals in *.
+      eapply eval_map_ex.
+      + exact H3.
+      + exact H4.
+      + exact H5.
+      + reflexivity.
+      + exact H7.
+      + intros.
+        pose (H8 j H2). apply H0 in e. exact e.
+        rewrite length_make_map_exps. lia.
+      + apply H0 in H11. auto. rewrite length_make_map_exps. lia.
+  }
+  split; intros.
+  * eapply A. exact H. auto. auto.
+  * eapply A. symmetry. exact H.
+    simpl. simpl in H0. rewrite length_make_map_exps. rewrite length_make_map_exps in H0.
+    intros. apply weak_sym. apply H0. lia. auto.
+Qed.
+
+Theorem ETry_weak_congr (e1 e2 e3 : Expression) vl1 vl2 : forall (e1' e2' e3' : Expression),
+  weakly_equivalent e1 e1' ->
+  weakly_equivalent e2 e2' ->
+  weakly_equivalent e3 e3'
+->
+  weakly_equivalent_single (ETry e1 vl1 e2 vl2 e3) (ETry e1' vl1 e2' vl2 e3').
+Proof.
+  assert (A : forall e1 e1' e2 e2' e3 e3' env id eff id' res eff',
+    weakly_equivalent e1 e1' ->
+    weakly_equivalent e2 e2' ->
+    weakly_equivalent e3 e3' ->
+    |env, id, ETry e1 vl1 e2 vl2 e3, eff | -s> |id', res, eff'|
+    ->
+    |env, id, ETry e1' vl1 e2' vl2 e3', eff| -s> |id', res, eff'|
+  ).
+  {
+    intros. inversion H2; subst.
+    * eapply eval_try. apply H. exact H14. auto. apply H0. exact H16.
+    * eapply eval_catch. apply H. exact H14. apply H1. exact H15.
+  }
+  split; intros.
+  * eapply A. exact H. exact H0. exact H1. auto.
+  * eapply A.
+    1-3: apply weak_sym.
+    exact H. exact H0. exact H1. auto.
+Qed.
+
+Theorem EValues_weak_congr (l : list SingleExpression) : forall (l' : list SingleExpression),
+  length l = length l' ->
+  (forall i, i < length l -> weakly_equivalent_single (nth i l ErrorExp) (nth i l' ErrorExp))
+->
+  weakly_equivalent (EValues l) (EValues l').
+Proof.
+  assert (A : forall (l l' : list SingleExpression) env id eff id' res eff',
+    length l = length l' ->
+    (forall i, i < length l -> weakly_equivalent_single (nth i l ErrorExp) (nth i l' ErrorExp))
+    ->
+    |env, id, EValues l, eff| -e> |id', res, eff'|
+    ->
+    |env, id, EValues l', eff| -e> |id', res, eff'|). {
+  intros. unfold weakly_equivalent, weakly_equivalent_single in *.
+  * inversion H1; subst; rewrite H in *.
+    - eapply eval_values.
+      + exact H3.
+      + exact H4.
+      + exact H5.
+      + intros. pose (H6 i H2). apply H0 in e. 2: auto. auto.
+      + auto.
+      + auto.
+    - eapply eval_values_ex.
+      + exact H3.
+      + reflexivity.
+      + exact H5.
+      + exact H6.
+      + intros. pose (H7 j H2). apply H0 in e. 2: lia. auto.
+      + apply H0 in H10. auto. lia.
+  }
+  split; intros.
+  * eapply A. exact H. auto. auto.
+  * eapply A. symmetry. exact H. intros. rewrite <- H in *.
+    apply weakly_equivalent_single_sym. auto. auto.
+Qed.
+
+Theorem ESingle_weak_congr (e : SingleExpression)  : forall (e': SingleExpression),
+  weakly_equivalent_single e e'
+->
+  weakly_equivalent (ESingle e) (ESingle e').
+Proof.
+  unfold weakly_equivalent_single.
+  split; intros.
+  * inversion H0. subst. destruct H. apply H in H4. destruct H4, H2.
+    exists x. split; auto. eapply eval_single; auto.
+  * inversion H0. subst. destruct H. apply H1 in H4. destruct H4, H2.
+    exists x. split; auto. eapply eval_single; auto.
 Qed.
 
 End congruence.
